src/MMIOTrace.v
@@ -1,0 +1,6 @@
+Require Import riscv.util.Word.
+Require Import riscv.Utility.
+
+Inductive MMIOAction := MMInput | MMOutput.
+
+Definition MMIOEvent(Addr: Set): Set := MMIOAction * Addr * word 32.
